<?xml version="1.0" encoding="UTF-8"?>
<!-- Changelog -->
<!-- 12/05/14 - created -->

<rdf:RDF
	xmlns:dc="http://purl.org/dc/elements/1.1/"
	xmlns:dcterms="http://purl.org/dc/terms/"
	xmlns:owl="http://www.w3.org/2002/07/owl#"
	xmlns:rdf="http://www.w3.org/1999/02/22-rdf-syntax-ns#"
	xmlns:rdfs="http://www.w3.org/2000/01/rdf-schema#"
	xmlns:role="http://purl.org/role/terms/">

    <owl:Ontology rdf:about="http://scam.sf.net/schema#">
      <dcterms:title xml:lang="en">ReM3 Model</dcterms:title>
      <owl:versionInfo>version 0.1</owl:versionInfo>
      <dcterms:description xml:lang="en">ReM2 Model used for the EntryStore system.</dcterms:description>
      <rdfs:seeAlso rdf:resource="http://code.google.com/p/entrystore/" rdfs:label="EntryStore project Homepage"/>
    </owl:Ontology>

    <!-- CLASSES ResourceType-->
    <rdfs:Class rdf:about="http://scam.sf.net/schema#InformationResource">
      <rdfs:label>Information Resource</rdfs:label>
      <rdfs:comment>A resource that has a retrievable representation.</rdfs:comment>
    </rdfs:Class>
    <rdfs:Class rdf:about="http://scam.sf.net/schema#NamedResource">
      <rdfs:label>Named Resource</rdfs:label>
      <rdfs:comment>A resource that is not an information resource, that is, have no retrievable representation.</rdfs:comment>
    </rdfs:Class>

    <!-- CLASSES GraphType-->
    <rdfs:Class rdf:about="http://scam.sf.net/schema#Graph">
      <rdfs:label>Graph</rdfs:label>
      <rdfs:comment>A retrivable RDF Graph.</rdfs:comment>
      <rdfs:subClassOf rdf:resource="http://scam.sf.net/schema#InformationResource"/>
    </rdfs:Class>
    <rdfs:Class rdf:about="http://scam.sf.net/schema#Entry">
      <rdfs:label>Entry</rdfs:label>
      <rdfs:comment>An entry expressed as an RDF graph, including references to a resource, 
      resource metadata, external metadata, and cached external metadata. 
      The entry also contains access control information and provenance information.</rdfs:comment>
      <rdfs:subClassOf rdf:resource="http://scam.sf.net/schema#Graph"/>
    </rdfs:Class>
    <rdfs:Class rdf:about="http://scam.sf.net/schema#List">
      <rdfs:label>List</rdfs:label>
      <rdfs:comment>A list of entries expressed as an RDF graph containing an rdf:Seq ordering the entries</rdfs:comment>
      <rdfs:subClassOf rdf:resource="http://scam.sf.net/schema#Graph"/>
    </rdfs:Class>
    <rdfs:Class rdf:about="http://scam.sf.net/schema#User">
      <rdfs:label>User</rdfs:label>
      <rdfs:comment>A user expressed as an RDF graph.</rdfs:comment>
      <rdfs:subClassOf rdf:resource="http://scam.sf.net/schema#Graph"/>
    </rdfs:Class>
    <rdfs:Class rdf:about="http://scam.sf.net/schema#Group">
      <rdfs:label>Group</rdfs:label>
      <rdfs:comment>A group expressed as as a list of Entries corresponding to users. 
      The group is expressedan as an RDF graph containing a rdf:Seq pointing to the entries.</rdfs:comment>
      <rdfs:subClassOf rdf:resource="http://scam.sf.net/schema#List"/>
    </rdfs:Class>
    <rdfs:Class rdf:about="http://scam.sf.net/schema#String">
      <rdfs:label>String</rdfs:label>
      <rdfs:comment>An string expressed as a single statement in an RDF graph.
      The subject of the statement is the URI to the information resource holding the RDF graph
      the predicate is rdf:value and the object is the string itself.</rdfs:comment>
      <rdfs:subClassOf rdf:resource="http://scam.sf.net/schema#Graph"/>
    </rdfs:Class>
    <rdfs:Class rdf:about="http://scam.sf.net/schema#Context">
      <rdfs:label>Context</rdfs:label>
      <rdfs:comment>A context is a set of entries expressed as an RDF graph containing relations to all its contained Entries.</rdfs:comment>
      <rdfs:subClassOf rdf:resource="http://scam.sf.net/schema#Graph"/>
    </rdfs:Class>
    
    <!-- CLASSES EntryType-->
    <rdfs:Class rdf:about="http://scam.sf.net/schema#Local">
      <rdfs:label>Local entry</rdfs:label>
      <rdfs:comment>A local entry, that is where the resource is contained in the same system as the entry itself.</rdfs:comment>
      <rdfs:subClassOf rdf:resource="http://scam.sf.net/schema#Entry"/>
    </rdfs:Class>
    <rdfs:Class rdf:about="http://scam.sf.net/schema#Link">
      <rdfs:label>Link entry</rdfs:label>
      <rdfs:comment>A link entry is an entry where the resource is external, that is, 
      not contained in the same system (or context) as the entry itself. 
      Typically links to webpages are modeled as link entries.</rdfs:comment>
      <rdfs:subClassOf rdf:resource="http://scam.sf.net/schema#Entry"/>
    </rdfs:Class>
    <rdfs:Class rdf:about="http://scam.sf.net/schema#Reference">
      <rdfs:label>Reference entry</rdfs:label>
      <rdfs:comment>A reference entry is an entry where both the metadata and the resource are external, that is,
      not contained in the system (or context) as the entry itself. 
      The external metadata is pointed to via the externalMetadata property and if there is a local cache of the
      external metadata it is pointed to via the cachedExternalMetadata property.
      Typically library resources are suitable to describe as reference entries.</rdfs:comment>
      <rdfs:subClassOf rdf:resource="http://scam.sf.net/schema#Entry"/>
    </rdfs:Class>
    <rdfs:Class rdf:about="http://scam.sf.net/schema#LinkReference">
      <rdfs:label>Link-reference entry</rdfs:label>
      <rdfs:comment>A link-reference entry is an reference entry that also has metadata locally.
      Such local metadata typically complements the external metadata.</rdfs:comment>
      <rdfs:subClassOf rdf:resource="http://scam.sf.net/schema#Link"/>
      <rdfs:subClassOf rdf:resource="http://scam.sf.net/schema#Reference"/>
    </rdfs:Class>
    
    
    <!--#####     PROPERTIES    ####  -->
    <rdfs:Property rdf:about="http://scam.sf.net/schema#resource">
      <rdfs:label>resource</rdfs:label>
      <rdfs:comment>Indicates the resource belonging to an entry.</rdfs:comment>
      <rdfs:domain rdf:resource="http://scam.sf.net/schema#Entry"/>
      <rdfs:range rdf:resource="http://www.w3.org/1999/02/22-rdf-syntax-ns#Resource"/>
    </rdfs:Property>
    <rdfs:Property rdf:about="http://scam.sf.net/schema#metadata">
      <rdfs:label>metadata</rdfs:label>
      <rdfs:comment>Indicates the local metadata of an entry.</rdfs:comment>
      <rdfs:domain rdf:resource="http://scam.sf.net/schema#Entry"/>
      <rdfs:range rdf:resource="http://scam.sf.net/schema#Graph"/>
    </rdfs:Property>
    <rdfs:Property rdf:about="http://scam.sf.net/schema#externalMetadata">
      <rdfs:label>external metadata</rdfs:label>
      <rdfs:comment>Indicates the external metadata of a reference entry.</rdfs:comment>
      <rdfs:domain rdf:resource="http://scam.sf.net/schema#ReferenceEntry"/>
      <rdfs:range rdf:resource="http://www.w3.org/1999/02/22-rdf-syntax-ns#Resource"/>
    </rdfs:Property>
    <rdfs:Property rdf:about="http://scam.sf.net/schema#cachedExternalMetadata">
      <rdfs:label>cached external metadata</rdfs:label>
      <rdfs:comment>Indicates the cached external metadata of a reference entry.</rdfs:comment>
      <rdfs:domain rdf:resource="http://scam.sf.net/schema#ReferenceEntry"/>
      <rdfs:range rdf:resource="http://scam.sf.net/schema#Graph"/>
    </rdfs:Property>
</rdf:RDF>